define an ifc_seq rule, and start proving it, but since star does not mean "execute until done", but "execute for any number of steps", when we are given an execution of command "c1; c2", we do not know whether it stopped inside c1 or inside c2, and this makes the proof tricky

ifc/rules.v
@@ -10,6 +10,17 @@ Require Import lib.LibTactics.
 
 Local Open Scope logic.
 
+Definition ioverridePost{A: Type}(Q: A -> environ -> mpred)(R : A -> ret_assert): A -> ret_assert :=
+  fun (x: A) => (overridePost (Q x) (R x)).
+
+Ltac split_ifc_hyps :=
+  repeat match goal with
+  | H: ifc_def _ _ _ _ _ _ _ _ |- _ =>
+      let Hs := fresh H "s" in 
+      let Hi := fresh H "i" in
+      destruct H as [Hs Hi]
+  end.
+
 (* We need lifting on top of VST's lifting... *)
 
 Definition iand{A: Type}(P1: A -> pre_assert)(P2: A -> pre_assert): A -> pre_assert :=
@@ -20,6 +31,39 @@ Definition iprop{A: Type}(P: pre_assert): A -> pre_assert := fun (_: A) => P.
 Section RULES.
 Context (Espec : OracleKind).
 Context (CS: compspecs).
+
+Lemma ifc_seq{T: Type}:
+  forall Delta (P1 P2: T -> environ -> mpred) (P3: T -> ret_assert) h t
+    (N1 N2 N3: T -> stack_clsf) (A1 A2 A3: T -> heap_clsf),
+  ifc_def Delta P1 N1 A1 h (ioverridePost P2 P3) N2 A2 ->
+  ifc_def (update_tycon Delta h) P2 N2 A2 t P3 N3 A3 ->
+  ifc_def Delta P1 N1 A1 (Ssequence h t) P3 N3 A3.
+Proof.
+  introv H1 H2. split_ifc_hyps. split.
+  - intro. apply* semax_seq.
+  - unfold ifc_core, simple_ifc in *.
+    intros x x' ge e1 e1' te1 te1' s3 s3' m1 m3 m1' m3' n.
+    intros Sat1 Sat1' SE1 HE1 Star1 Star1'.
+    destruct n as [|n].
+    + (* 0 steps *)
+      inversion Star1. subst s s3 m m3.
+      inversion Star1'. subst s s3' m m3'.
+      specialize (H1i x x' ge e1 e1' te1 te1').
+      specialize (H1i (State e1 te1 (Kseq h :: nil)) (State e1' te1' (Kseq h :: nil))).
+(*
+      specialize (H1i m1 m1 m1' m1' 0 Sat1 Sat1').
+      specialize (H1i (stack_lo_equiv_change_cmd _ _ _ _ _ _ _ _ _ _ SE1) HE1).
+      specialize (H1i (star_refl _ _ _) (star_refl _ _ _)).
+      destruct H1i as [SE2 HE2].
+      specialize (H2i x x' ge e1 e1' te1 te1').
+      specialize (H2i (State e1 te1 (Kseq h :: nil)) (State e1' te1' (Kseq h :: nil))).
+*)
+
+(* star does not mean "execute until done", so execution can be anywhere inside h or t,
+   which seems difficult to reason about!
+   TODO first just define exec to go until empty cont list *)
+
+Admitted.
 
 Lemma ifc_ifthenelse: forall {T: Type} (Delta: tycontext) 
   (P: T -> pre_assert) (N: T -> stack_clsf) (A: T -> heap_clsf)
